access-control, infoflow: use generic relation for pasDomainAbs
This patch generalises the mapping between authority labels and
scheduler domains, so that the access-control integrity property still
holds when labels are not partitioned into domains. This lets us use
the integrity result on systems that don't use the domain scheduler.

The information flow proofs still rely on the domain partitioning,
hence we add constraints on the label-domain mapping for the info-flow
results to hold.

Jira VER-945

proof/access-control/Syscall_AC.thy
@@ -262,8 +262,11 @@ declare hoare_post_taut [simp del]
 
 crunch pas_cur_domain[wp]: as_user "pas_cur_domain aag"
 
-definition guarded_pas_domain where
-"guarded_pas_domain aag \<equiv> \<lambda>s. cur_thread s \<noteq> idle_thread s \<longrightarrow> pasDomainAbs aag (cur_domain s) = pasObjectAbs aag (cur_thread s)"
+definition guarded_pas_domain
+  where
+  "guarded_pas_domain aag \<equiv>
+     \<lambda>s. cur_thread s \<noteq> idle_thread s \<longrightarrow>
+         pasObjectAbs aag (cur_thread s) \<in> pasDomainAbs aag (cur_domain s)"
 
 
 lemma guarded_pas_domain_lift:
@@ -832,36 +835,27 @@ lemma switch_to_thread_respects:
   apply (wp | simp add: clearExMonitor_def)+
   done
 
+text {*
+Variants of scheduling lemmas without is_subject assumption.
+See comment for @{thm tcb_sched_action_dequeue_integrity'}
+*}
+(* FIXME: replace switch_to_thread_respects above (used in infoflow/ADT_IF) *)
+lemma switch_to_thread_respects':
+  "\<lbrace>integrity aag X st and pas_refined aag
+    and (\<lambda>s. pasSubject aag \<in> pasDomainAbs aag (tcb_domain (the (ekheap s t)))) \<rbrace>
+  switch_to_thread t
+  \<lbrace>\<lambda>rv. integrity aag X st\<rbrace>"
+  unfolding switch_to_thread_def arch_switch_to_thread_def
+  apply (simp add: spec_valid_def)
+  apply (wp tcb_sched_action_dequeue_integrity' | simp add: clearExMonitor_def)+
+  done
+
 lemma switch_to_idle_thread_respects:
   "\<lbrace>integrity aag X st\<rbrace>
     switch_to_idle_thread
   \<lbrace>\<lambda>rv. integrity aag X st\<rbrace>"
   unfolding switch_to_idle_thread_def arch_switch_to_idle_thread_def
   by (wp | simp)+
-
-lemma max_non_empty_queue_is_subject:
-  "\<lbrakk>tcb_domain_map_wellformed aag s;
-    st_tcb_at (op = sta) (hd (max_non_empty_queue (ready_queues s (cur_domain s)))) s;
-    pas_cur_domain aag s; valid_queues s;ready_queues s (cur_domain s) prio \<noteq> [];
-    runnable sta\<rbrakk>
-   \<Longrightarrow> is_subject aag (hd (max_non_empty_queue (ready_queues s (cur_domain s))))"
-  apply (clarsimp simp: tcb_domain_map_wellformed_aux_def)
-  apply (erule_tac x="(hd (max_non_empty_queue (ready_queues s (cur_domain s))), cur_domain s)" in ballE)
-   apply simp
-  apply (clarsimp simp: valid_queues_def is_etcb_at_def)
-  apply (erule_tac x="cur_domain s" in allE)
-  apply (erule_tac x="Max {prio. ready_queues s (cur_domain s) prio \<noteq> []}" in allE)
-  apply clarsimp
-  apply (erule_tac x="hd (max_non_empty_queue (ready_queues s (cur_domain s)))" in ballE)
-   apply (clarsimp)
-   apply (erule notE, rule domtcbs)
-    apply force
-   apply (simp add: etcb_at_def)
-  apply (simp add: max_non_empty_queue_def)
-  apply (erule_tac P="hd A \<in> B" for A B in notE)
-  apply (rule Max_prop)
-   apply force+
-  done
 
 lemma choose_thread_respects_pasMayEditReadyQueues:
   "\<lbrace>integrity aag X st and pas_refined aag and einvs and valid_queues and K (pasMayEditReadyQueues aag ) \<rbrace>
@@ -875,24 +869,25 @@ lemma choose_thread_respects:
   "\<lbrace>integrity aag X st and pas_refined aag and pas_cur_domain aag and einvs and valid_queues\<rbrace>
    choose_thread
    \<lbrace>\<lambda>rv. integrity aag X st\<rbrace>"
-  apply (simp add: choose_thread_def guarded_switch_to_def | wp switch_to_thread_respects switch_to_idle_thread_respects gts_wp)+
+  apply (simp add: choose_thread_def guarded_switch_to_def
+        | wp switch_to_thread_respects' switch_to_idle_thread_respects gts_wp)+
   apply (clarsimp simp: pas_refined_def)
   apply (clarsimp simp: tcb_domain_map_wellformed_aux_def)
-  apply (erule_tac x="(hd (max_non_empty_queue (ready_queues s (cur_domain s))), cur_domain s)" in ballE)
-   apply simp
   apply (clarsimp simp: valid_queues_def is_etcb_at_def)
   apply (erule_tac x="cur_domain s" in allE)
   apply (erule_tac x="Max {prio. ready_queues s (cur_domain s) prio \<noteq> []}" in allE)
   apply clarsimp
   apply (erule_tac x="hd (max_non_empty_queue (ready_queues s (cur_domain s)))" in ballE)
-   apply (clarsimp)
-   apply (erule notE, rule domtcbs)
-    apply force
-   apply (simp add: etcb_at_def)
-  apply (simp add: max_non_empty_queue_def)
-  apply (erule_tac P="hd A \<in> B" for A B in notE)
-  apply (rule Max_prop)
-   apply force+
+   apply (clarsimp simp: etcb_at_def)
+  (* thread we're switching to is in cur_domain *)
+  apply (rule_tac s = "cur_domain s" in subst)
+  apply (clarsimp simp: max_non_empty_queue_def)
+   apply (frule tcb_at_ekheap_dom[OF st_tcb_at_tcb_at])
+    apply (simp add: valid_sched_def)
+   apply (clarsimp simp: max_non_empty_queue_def)
+   apply (metis (mono_tags, lifting) setcomp_Max_has_prop hd_in_set)
+  (* pas_cur_domain *)
+  apply assumption
   done
 
 lemma guarded_switch_to_respects:
@@ -937,18 +932,23 @@ lemma next_domain_valid_sched:
 crunch current_ipc_buffer_register [wp]: tcb_sched_action "\<lambda>s. P (current_ipc_buffer_register s)"
    (wp: crunch_wps without_preemption_wp simp: crunch_simps current_ipc_buffer_register_def get_tcb_def)
 
-lemma valid_sched_action_switch_is_subject:
-  "\<lbrakk> scheduler_action s = switch_thread t ; valid_sched_action s ;
-     valid_etcbs s ; pas_refined aag s ; pas_cur_domain aag s \<rbrakk>
-   \<Longrightarrow> is_subject aag t"
-  apply (clarsimp simp: valid_sched_def valid_sched_action_def weak_valid_sched_action_2_def
+text {*
+We need to use the domain of t instead of @{term "is_subject aag t"}
+because t's domain may contain multiple labels. See the comment for
+@{thm tcb_sched_action_dequeue_integrity'}
+*}
+lemma valid_sched_action_switch_subject_thread:
+   "\<lbrakk> scheduler_action s = switch_thread t ; valid_sched_action s ;
+      valid_etcbs s ; pas_refined aag s ; pas_cur_domain aag s \<rbrakk>
+    \<Longrightarrow> pasObjectAbs aag t \<in> pasDomainAbs aag (tcb_domain (the (ekheap s t))) \<and>
+        pasSubject aag \<in> pasDomainAbs aag (tcb_domain (the (ekheap s t)))"
+  apply (clarsimp simp: valid_sched_action_def weak_valid_sched_action_2_def
                         switch_in_cur_domain_2_def in_cur_domain_2_def valid_etcbs_def
-                        etcb_at_def st_tcb_at_def obj_at_def is_etcb_at_def split: option.splits)
-   apply force
-  apply (clarsimp simp: pas_refined_def tcb_domain_map_wellformed_aux_def)
-  apply (drule_tac x="(t, cur_domain s)" in bspec)
-   apply (force intro: domtcbs)
-  apply clarsimp
+                        etcb_at_def st_tcb_at_def obj_at_def is_etcb_at_def)
+  apply (rule conjI)
+   apply (force simp: pas_refined_def tcb_domain_map_wellformed_aux_def
+                intro: domtcbs)
+  apply force
   done
 
 
@@ -972,17 +972,18 @@ lemma schedule_integrity:
   apply (rule hoare_pre)
   supply ethread_get_wp[wp del]
   apply (wp|wpc|simp only: schedule_choose_new_thread_def)+
-  apply (wpsimp wp: alternative_wp switch_to_thread_respects select_wp switch_to_idle_thread_respects
+  apply (wpsimp wp: alternative_wp switch_to_thread_respects' select_wp switch_to_idle_thread_respects
                  guarded_switch_to_lift choose_thread_respects gts_wp hoare_drop_imps
                  set_scheduler_action_cnt_valid_sched append_thread_queued enqueue_thread_queued
                  tcb_sched_action_enqueue_valid_blocked_except
+                 tcb_sched_action_append_integrity'
             wp_del: ethread_get_wp
     | wpc
     | simp add: allActiveTCBs_def schedule_choose_new_thread_def
     | rule hoare_pre_cont[where a=next_domain])+
   apply (auto simp: obj_at_def st_tcb_at_def not_cur_thread_2_def valid_sched_def
               valid_sched_action_def weak_valid_sched_action_def
-              valid_sched_action_switch_is_subject schedule_choose_new_thread_def)
+              valid_sched_action_switch_subject_thread schedule_choose_new_thread_def)
   done
 
 lemma  valid_sched_valid_sched_action:
